Prove (1) ==> (2) and begin proof of (3) ==> (1)

Escallon/LR_Parsing/LR_Parser.thy
@@ -17,11 +17,11 @@ definition char_fa :: "(('n, 't) sym, ('n, 't) item) nfa" where
       P = Prods G';
       Q = It G';
       F = {[X \<rightarrow> \<alpha> . []] |X \<alpha>. [X \<rightarrow> \<alpha> . []] \<in> It G'};
-      \<delta> = (\<lambda>s a. case s of 
+      \<Delta> = (\<lambda>s a. case s of 
         [X \<rightarrow> \<alpha> . Y # \<beta>]  \<Rightarrow> if a = Y \<and> (X, \<alpha>@Y#\<beta>) \<in> P then {[X \<rightarrow> \<alpha>@[Y] . \<beta>]} else {}| 
          _ \<Rightarrow> {}); 
       \<E> = {([X \<rightarrow> \<alpha> . Nt Y # \<beta>], [Y \<rightarrow> [] . \<gamma>]) | X \<alpha> Y \<beta> \<gamma>. (X, \<alpha> @Nt Y#\<beta>) \<in> P \<and> (Y, \<gamma>) \<in> P} in
-    \<lparr>nfa.states = Q, nfa.init = {[S' \<rightarrow> [] . [Nt S]]}, nfa.final = F, nfa.nxt = \<delta>, nfa.eps = \<E>\<rparr>"
+    \<lparr>nfa.states = Q, nfa.init = {[S' \<rightarrow> [] . [Nt S]]}, nfa.final = F, nfa.nxt = \<Delta>, nfa.eps = \<E>\<rparr>"
 
 lemma states_char_fa [simp]: 
   "nfa.states char_fa = It G'"
@@ -37,14 +37,46 @@ lemma final_char_fa [simp]:
 
 lemma nxt_char_fa [simp]:
   "nfa.nxt char_fa = (\<lambda>s a. case s of 
-        [X \<rightarrow> \<alpha> . Y # \<beta>]  \<Rightarrow> if a = Y \<and> ((X, \<alpha> @ (Y#\<beta>)) \<in> Prods G') then {[X \<rightarrow> \<alpha> @ [Y] . \<beta>]} else {}| 
-        _ \<Rightarrow> {})"
+        [X \<rightarrow> \<alpha> . Y # \<beta>]  \<Rightarrow> if a = Y \<and> ((X, \<alpha> @ Y # \<beta>) \<in> Prods G') then {[X \<rightarrow> \<alpha> @ [Y] . \<beta>]} 
+  else {} | _ \<Rightarrow> {})"
   unfolding char_fa_def by (meson nfa.select_convs(4))
+
+lemma char_fa_nxt_neq_or_not_Prod_imp_empty:
+  assumes "Y \<noteq> a \<or> (X, \<alpha> @ Y # \<beta>) \<notin> Prods G'"
+  shows "nfa.nxt char_fa ([X \<rightarrow> \<alpha> . Y # \<beta>]) a = {}" 
+  using assms by auto
+
+lemma char_fa_nxt_in_Prods_imp_singleton:
+  assumes "(X, \<alpha> @ Y # \<beta>) \<in> Prods G'"
+  shows "nfa.nxt char_fa ([X \<rightarrow> \<alpha> . Y # \<beta>]) Y = {[X \<rightarrow> \<alpha> @ [Y] . \<beta>]}"
+  using assms by simp
+
+lemma char_fa_nxt_nempty_imp_hd:
+  assumes "nfa.nxt char_fa ([X \<rightarrow> \<alpha> . \<beta>]) a \<noteq> {}" 
+  obtains \<gamma> where "\<beta> = a # \<gamma>" "(X, \<alpha>@\<beta>) \<in> Prods G'"
+  using assms 
+  by (metis (lifting) char_fa_nxt_neq_or_not_Prod_imp_empty item.case list.exhaust list.simps(4)
+      nxt_char_fa)
+
+lemma in_char_fa_nxt_imp_shift:
+  assumes "q \<in> nfa.nxt char_fa p a"
+  obtains X \<alpha> \<beta> where "p = [X \<rightarrow> \<alpha> . a # \<beta>]" "q = [X \<rightarrow> \<alpha> @ [a] . \<beta>]"
+proof -
+  obtain X \<alpha> \<beta> Y \<gamma> \<delta> where pq_defs: "p = [X \<rightarrow> \<alpha> . \<beta>]" "q = [Y \<rightarrow> \<gamma> . \<delta>]" 
+    using item.exhaust by meson
+  moreover with char_fa_nxt_nempty_imp_hd assms obtain \<zeta> where "\<beta> = a # \<zeta>" "(X, \<alpha>@\<beta>) \<in> Prods G'" 
+    by blast
+  moreover with char_fa_nxt_in_Prods_imp_singleton have "q = [X \<rightarrow> \<alpha> @ [a] . \<zeta>]"
+    using assms pq_defs(1) by blast
+  ultimately show thesis using that by presburger
+qed
 
 lemma eps_char_fa [simp]:
   "nfa.eps char_fa 
     = {([X \<rightarrow> \<alpha> . Nt Y # \<beta>], [Y \<rightarrow> [] . \<gamma>]) | X \<alpha> Y \<beta> \<gamma>. (X, \<alpha> @ Nt Y # \<beta>) \<in> Prods G' \<and> (Y, \<gamma>) \<in> Prods G'}"
   unfolding char_fa_def by (meson nfa.select_convs(5))
+
+
 
 sublocale char_fa: nfa char_fa 
 proof (unfold_locales, goal_cases 1 2 nxt_closed 3)
@@ -56,9 +88,11 @@ proof (unfold_locales, goal_cases 1 2 nxt_closed 3)
   proof cases
     case eq
     then show ?thesis 
-      using eq nxt_closed q_def by cases (auto simp: It_defs)
+      using nxt_closed q_def by (auto simp: It_defs)
   qed (use nxt_closed q_def in fastforce)+
 qed (use G'_def It_defs It_finite[OF G'_finite] in fastforce)+
+
+
 
 definition LR\<^sub>0 :: "(('n, 't) sym, ('n, 't) item set) dfa" where
   "LR\<^sub>0 \<equiv> nfa.Power_dfa char_fa"
@@ -66,9 +100,10 @@ definition LR\<^sub>0 :: "(('n, 't) sym, ('n, 't) item set) dfa" where
 sublocale canon_LR0: dfa LR\<^sub>0
   unfolding LR\<^sub>0_def by (rule char_fa.dfa_Power)
 
-
 end
 
+
+ 
 
 section \<open>NFA Configurations and Steps\<close>
 
@@ -104,6 +139,48 @@ lemma steps_len_dec:
   "(p,u) \<turnstile>* (q,v) \<Longrightarrow> length u \<ge> length v" 
   by (induction "(p,u)" "(q,v)" arbitrary: q v rule: rtranclp.induct)
   (use step_len_dec surj_pair le_trans in fastforce)+
+
+lemma nxt_indep:
+  assumes "(p, a # u) \<turnstile> (q, u)"
+  shows "(p, a # v) \<turnstile> (q, v)"
+  using assms by auto
+
+lemma eps_indep:
+  assumes "(p, u) \<turnstile> (q, u)"
+  shows "(p, v) \<turnstile> (q, v)"
+  using assms by blast
+
+lemma step_imp_nempty_or_eq:
+  assumes "(p, u) \<turnstile> (q, v)"
+  shows "u \<noteq> [] \<or> u = v"
+  using assms by cases auto
+
+lemma stepn_indep:
+  assumes "(p, u@v) \<turnstile>(n) (q, v)"
+  shows "(p, u@w) \<turnstile>(n) (q, w)"
+  using assms proof (induction n arbitrary: p u q)
+  case 0
+  then show ?case by simp
+next
+  case (Suc n)
+  then obtain r x where n_steps: "(p, u@v) \<turnstile> (r, x)" "(r, x) \<turnstile>(n) (q, v)" 
+    by (metis eq_fst_iff relpowp_Suc_D2)
+  from this(1) show ?case 
+  proof cases
+    case (nxt a)
+    then obtain y where u_decomp: "u = a # y" "x = y @ v" using n_steps 
+      by (metis append_eq_Cons_conv impossible_Cons relpowp_imp_rtranclp steps_len_dec)
+    hence "(p, u @ w) \<turnstile> (r, y @ w)" by (simp add: nxt(2) step.nxt)
+    also note Suc.IH[OF n_steps(2)[unfolded u_decomp(2)]]
+    finally show ?thesis .
+  next
+    case eps
+    with Suc.IH n_steps(2) have "(r, u @ w) \<turnstile>(n) (q, w)" by blast
+    then show ?thesis using eps_indep[OF n_steps(1)[unfolded eps(1)], of "u @ w"] 
+      by (meson relpowp_Suc_I2)
+  qed
+qed
+
 
 section \<open>\<epsilon>-Transitions\<close>
 
@@ -158,7 +235,6 @@ lemma last_eps_step:
 qed
 
 
-
 lemma noeps_eps_stepn_eq:
   "\<lbrakk>c1 \<turnstile>\<epsilon>(n) c2; c0 \<turnstile>\<epsilon>(0) c1\<rbrakk> \<Longrightarrow> c0 \<turnstile>\<epsilon>(n) c2"
 proof (induction rule: eps_stepn.induct)
@@ -207,22 +283,19 @@ end
 
 section \<open>Proving 3.4.1\<close>
 
-
-
-
 context Extended_Cfg
 begin
 
-
-interpretation I: ipda G IPDA 
+interpretation P: ipda G IPDA 
   by standard simp
 
 corollary ipda_IPDA: 
   "ipda G IPDA"
-  by (rule I.ipda_axioms)
+  by (rule P.ipda_axioms)
 
 notation char_fa.step (infix \<open>\<turnstile>c\<close> 70)
 notation char_fa.steps (infix \<open>\<turnstile>c*\<close> 70)
+notation char_fa.stepn (\<open>_ \<turnstile>c'(_') _\<close> 70)
 notation char_fa.eps_stepn (\<open>_ \<turnstile>c\<epsilon>'(_') _\<close> 70)
 
 type_synonym ('q,'s) ipda_config = "('q,'s) item list \<times> 's list"
@@ -239,50 +312,112 @@ abbreviation IPDA_stepn :: "('n,'t) item list \<times> 't list \<Rightarrow> nat
                     \<Rightarrow> bool" ( \<open>_ \<turnstile>P'(_') _\<close> 70) where
   "c0 \<turnstile>P(n) c1 \<equiv> (ipda.stepn IPDA) c0 n c1"
 
-lemma deriver_imp_IPDA_comp:
-  assumes
-    "Prods G' \<turnstile> [Nt S'] \<Rightarrow>r \<alpha>@\<beta>"
-    "Prods G' \<turnstile> \<beta> \<Rightarrow>r* map Tm v"
-  shows
-    "([[S' \<rightarrow> \<alpha> . \<beta>], init_symbol IPDA], v) \<turnstile>P* ([I.final_state, init_symbol IPDA], [])"
-proof -
-  from assms have eq_S: "\<alpha>@\<beta> = [Nt S]" 
-    using S'_derive_imp_S append_eq_Cons_conv 
-    by (simp add: deriver_imp_derive)
-  then consider (left) "\<alpha> = [Nt S]" "\<beta> = []" | (right) "\<alpha> = []" "\<beta> = [Nt S]"
-    by (metis (no_types, opaque_lifting) Cons_eq_append_conv append_is_Nil_conv)
-  then show ?thesis 
+lemma char_step_cases[consumes 1, case_names nxt eps, cases set: char_fa.step]:
+  assumes "c0 \<turnstile>c c1"
+  obtains 
+    X \<alpha> Y \<beta> \<gamma> where "c0 = ([X \<rightarrow> \<alpha> . Y # \<beta>], Y # \<gamma>)" "c1 = ([X \<rightarrow> \<alpha> @ [Y] . \<beta>], \<gamma>)" 
+                      "(X, \<alpha> @ Y # \<beta>) \<in> Prods G'" |
+    X \<alpha> Y \<beta> \<delta> \<gamma> where "c0 = ([X \<rightarrow> \<alpha> . Nt Y # \<beta>], \<delta>)" "c1 = ([Y \<rightarrow> [] . \<gamma>], \<delta>)" "(Y, \<gamma>) \<in> Prods G'"
+                      "(X, \<alpha> @ Nt Y # \<beta>) \<in> Prods G'"
+  using assms proof cases
+  case (nxt q p a u)
+  then show ?thesis using that(1) in_char_fa_nxt_imp_shift char_fa_nxt_neq_or_not_Prod_imp_empty 
+    by (metis emptyE)
+next
+  case (eps p q w)
+  then show ?thesis unfolding eps_char_fa using that(2) by blast
+qed
+
+lemma char_reachable_imp_substring:
+  assumes "([S' \<rightarrow> [] . [Nt S]], \<gamma>) \<turnstile>c* ([A \<rightarrow> \<alpha> . \<beta>], \<delta>)"
+  obtains \<zeta> where "\<gamma> = \<zeta> @ \<alpha> @ \<delta>"
+  using assms proof (induction "([A \<rightarrow> \<alpha> . \<beta>], \<delta>)" arbitrary: A \<alpha> \<beta> \<delta> thesis rule: rtranclp_induct)
+  case base
+  then show ?case by simp
+next
+  case (step c)
+  from this(2) show ?case 
   proof cases
-    case left
-    with assms(2) have v_empty: "v = []" 
-      by (simp add: derivers_iff_derives)
-    then show ?thesis using eq_S left by simp
+    case (eps X \<alpha>' Y \<beta>' \<zeta> \<gamma>')
+    from step(3)[OF this(1)] obtain \<eta> where "\<gamma> = \<eta> @ \<alpha>' @ \<zeta>" .
+    then show ?thesis using eps step by auto
+  qed (use step in force)   
+qed
+
+
+lemma char_comp_imp_derivers:
+  assumes "([S' \<rightarrow> [] . [Nt S]], \<gamma>) \<turnstile>c* ([A \<rightarrow> \<alpha> . \<beta>], [])"
+  obtains \<gamma>' w where 
+    "Prods G' \<turnstile> [Nt S'] \<Rightarrow>r* \<gamma>' @ Nt A # map Tm w"
+    "Prods G' \<turnstile> \<gamma>' @ Nt A # map Tm w \<Rightarrow>r \<gamma>' @ \<alpha> @ \<beta> @ map Tm w"
+    "\<gamma> = \<gamma>' @ \<alpha>"
+proof -
+  from assms obtain n where "([S' \<rightarrow> [] . [Nt S]], \<gamma>) \<turnstile>c(n) ([A \<rightarrow> \<alpha> . \<beta>], [])"
+    using rtranclp_imp_relpowp by fast
+  with that show thesis
+  proof (induction n arbitrary: \<gamma> A \<alpha> \<beta> thesis)
+    case 0
+    then show ?case using 0(1)[of "[]" "[]"] G'_derive_S 
+      by (simp add: G'_def deriver_singleton)
   next
-    case right
-    with assms have "v \<in> LangS G'"  
-      using G'_derives_from_S_imp_in_Lang derivers_imp_derives by blast
-    then show ?thesis using eq_S I.Lang_def right 
-        I.Lang_eq_Lang_G Lang_preserved hist_singleton rtrancl_refl by auto
+    case (Suc n)
+    then obtain c where n_steps: "([S' \<rightarrow> [] . [Nt S]], \<gamma>) \<turnstile>c(n) c" "c \<turnstile>c ([A \<rightarrow> \<alpha> . \<beta>], [])" 
+      by auto
+    from this(2) show ?case 
+    proof cases
+      case (nxt X \<alpha>' Y \<beta>' \<gamma>')
+      moreover with n_steps obtain \<delta> where \<delta>_def: "\<gamma> = \<delta> @ \<alpha>' @ [Y]" 
+        using char_reachable_imp_substring[of \<gamma> X \<alpha>' "Y # \<beta>'" "[Y]"] relpowp_imp_rtranclp 
+        by (metis prod.inject)
+      ultimately have "([S' \<rightarrow> [] . [Nt S]], \<delta> @ \<alpha>') \<turnstile>c(n) ([X \<rightarrow> \<alpha>' . Y # \<beta>'], [])"
+        using n_steps nfa.stepn_indep[OF char_fa.nfa_axioms, of _ _ "\<delta> @ \<alpha>'" "[Y]" _ "[]"] 
+        by auto
+      from Suc.IH[OF _ this] obtain \<zeta> w where "Prods G' \<turnstile> [Nt S'] \<Rightarrow>r* \<zeta> @ Nt A # map Tm w"
+        "Prods G' \<turnstile> \<zeta> @ Nt A # map Tm w \<Rightarrow>r \<zeta> @ \<alpha>' @ Y # \<beta> @ map Tm w" "\<delta> @ \<alpha>' = \<zeta> @ \<alpha>'"
+        using nxt by auto
+      then show ?thesis using nxt Suc.prems(1) by (simp add: \<delta>_def)
+    next
+      case (eps X \<alpha>' Y \<beta>' \<delta> \<gamma>')
+      with n_steps Suc.IH[of X \<alpha>' "Nt Y # \<beta>'"] obtain \<zeta> w where X_deriv:
+        "Prods G' \<turnstile> [Nt S'] \<Rightarrow>r* \<zeta> @ Nt X # map Tm w"
+        "Prods G' \<turnstile> \<zeta> @ Nt X # map Tm w \<Rightarrow>r \<zeta> @ \<alpha>' @ Nt A # \<beta>' @ map Tm w" "\<gamma> = \<zeta> @ \<alpha>'"
+        by auto
+      moreover from this obtain v where \<beta>_deriv: "Prods G' \<turnstile> \<beta>' \<Rightarrow>r* map Tm v"
+        using reduced_derived_substring_imp_derives[OF _ G'_reduced G'_not_empty, of "\<zeta>@\<alpha>'@[Nt A]" \<beta>']
+          derivers_imp_derives
+        by (metis (no_types, opaque_lifting) Cfg.sel(2) G'_def append.assoc append_Cons append_Nil
+            derivers_iff_derives rtranclp.rtrancl_into_rtrancl)
+      have "Prods G' \<turnstile> [Nt S'] \<Rightarrow>r* \<gamma> @ Nt A # map Tm (v@w)"
+      proof -
+        note X_deriv(1)
+        also note X_deriv(2)
+        also from \<beta>_deriv have 
+          "Prods G' \<turnstile>  \<zeta> @ \<alpha>' @ Nt A # \<beta>' @ map Tm w \<Rightarrow>r*  \<zeta> @ \<alpha>' @ Nt A # map Tm (v@w)"
+          by (metis append_Cons append_Nil derivers_append_map_Tm derivers_prepend map_append)
+        finally show ?thesis using X_deriv(3) by simp
+      qed
+      moreover have "Prods G' \<turnstile> ... \<Rightarrow>r \<gamma> @ \<alpha> @ \<beta> @ map Tm (v@w)"
+        using eps(2,3) deriver.intros[of A "\<alpha>@\<beta>" _ \<gamma> "v@w"] by simp
+      ultimately show ?thesis using Suc.prems(1)[of \<gamma> "v@w"] eps by blast  
+    qed
   qed
 qed
 
-lemma char_comp_imp_derivers:
-  shows True sorry
 
 
-lemma derivers_imp_IPDA_comp:
+lemma derivers_imp_ipda_comp:
   assumes "Prods G' \<turnstile> [Nt S'] \<Rightarrow>r* \<gamma>@Nt A#map Tm w"
     "Prods G' \<turnstile> \<gamma>@Nt A#map Tm w \<Rightarrow>r \<gamma>@\<alpha>@\<beta>@map Tm w"
-    "Prods G' \<turnstile> \<beta> \<Rightarrow>r* map Tm v"
+    "Prods G' \<turnstile> \<beta> \<Rightarrow>* map Tm v"
   obtains \<rho> where 
-    "([A \<rightarrow> \<alpha> . \<beta>]#\<rho>@[init_symbol IPDA], v@w) \<turnstile>P* ([I.final_state, init_symbol IPDA], [])" 
+    "([A \<rightarrow> \<alpha> . \<beta>] # \<rho> @ [init_symbol IPDA], v@w) \<turnstile>P* ([P.final_state, init_symbol IPDA], [])" 
     "hist \<rho> = \<gamma>"
   using assms(1) proof cases
   case rtrancl_refl
   with assms have eqs: "\<gamma> = [] \<and> w = [] \<and> \<alpha>@\<beta> = [Nt S]" 
     using S'_derive_imp_S append_eq_Cons_conv deriver_imp_derive by fastforce
-  then show thesis using S'_derive_imp_S deriver_imp_IPDA_comp assms that 
-    by (metis I.hist_init I.init_symbol_ipda append.right_neutral append_Nil hist_singleton list.inject
+  then show thesis using S'_derive_imp_S P.deriver_imp_IPDA_comp assms that 
+    by (metis P.hist_init P.init_symbol_ipda append.right_neutral append_Nil hist_singleton list.inject
         rtrancl_refl sym.inject(1))
 next
   case (rtrancl_into_rtrancl b)
@@ -295,8 +430,8 @@ next
     case Nil
     then have eqs: "\<gamma> = [] \<and> w = [] \<and> \<alpha>@\<beta> = [Nt S] \<and> A = S'" 
       using S'_derive_imp_S append_eq_Cons_conv deriver_imp_derive by fastforce
-    then show thesis using S'_derive_imp_S deriver_imp_IPDA_comp Nil
-    by (metis I.hist_init I.init_symbol_ipda append.right_neutral append_Nil hist_singleton
+    then show thesis using S'_derive_imp_S P.deriver_imp_IPDA_comp Nil
+    by (metis P.hist_init P.init_symbol_ipda append.right_neutral append_Nil hist_singleton
         list.simps(8))
   next
     case (Cons i \<rho>)
@@ -311,21 +446,73 @@ next
       by (smt (verit, best) append.assoc append_same_eq map_append right_derivs_eq_imp_eq_tl)
     then obtain \<rho>' where \<rho>'_def:
       "([X \<rightarrow> \<alpha>' @ [Nt A] . \<beta>'] # \<rho>' @ [init_symbol IPDA], u@v') 
-          \<turnstile>P* ([I.final_state, init_symbol IPDA], [])"
+          \<turnstile>P* ([P.final_state, init_symbol IPDA], [])"
       "hist \<rho>' = \<alpha>''" 
       using Cons(1)[OF X_chain(1) rm_chain_imp_derivers[OF X_chain(1)], of "\<alpha>' @ [Nt A]" \<beta>']
-      by auto
+      by (metis append.assoc append_Cons append_Nil derivers_imp_derives)
     let ?\<rho> = "[X \<rightarrow> \<alpha>' . Nt A # \<beta>'] # \<rho>'"
     have hist_\<rho>: "hist ?\<rho> = \<gamma>" using X_chain(5) \<rho>'_def(2) by simp
-    from I.derives_imp_completes[OF Cons(5)[THEN derivers_imp_derives]] have 
+    from P.derives_imp_completes[OF Cons(5)] have 
       "([A \<rightarrow> \<alpha> . \<beta>] # ?\<rho> @ [init_symbol IPDA], v @ w) \<turnstile>P* ([A \<rightarrow> \<alpha>@\<beta> . []] # ?\<rho> @ [init_symbol IPDA], w)"
       by (metis append.right_neutral)
     also have "... \<turnstile>P ([X \<rightarrow> \<alpha>' @ [Nt A] . \<beta>'] # \<rho>' @ [init_symbol IPDA], u@v')"
       using X_chain(4) by auto
-    also have "... \<turnstile>P* ([I.final_state, init_symbol IPDA], [])" using \<rho>'_def by presburger
+    also have "... \<turnstile>P* ([P.final_state, init_symbol IPDA], [])" using \<rho>'_def by presburger
     finally show ?case using hist_\<rho> Cons(6) by presburger
   qed
 qed 
+
+
+lemma ipda_reaches_final_imp_rm_chain:
+  assumes "([A \<rightarrow> \<alpha> . \<beta>] # \<rho> @ [init_symbol IPDA], w) \<turnstile>P* ([P.final_state, init_symbol IPDA], [])"
+  obtains "\<rho> = []" |
+    \<sigma> X \<alpha>' \<beta>' \<gamma> where "\<rho> = [X \<rightarrow> \<alpha>' . Nt A # \<beta>'] # \<sigma>" "Prods G' \<Turnstile> [Nt S'] \<Rightarrow>r* \<rho> \<Rightarrow>r* \<gamma>"
+  sorry
+
+
+lemma ipda_comp_imp_char_comp:
+  assumes "([A \<rightarrow> \<alpha> . \<beta>] # \<rho> @ [init_symbol IPDA], w) \<turnstile>P* ([P.final_state, init_symbol IPDA], [])"
+  shows "([S' \<rightarrow> [] . [Nt S]], hist \<rho> @ \<alpha>) \<turnstile>c* ([A \<rightarrow> \<alpha> . \<beta>], [])"
+proof -
+  from ipda_reaches_final_imp_rm_chain[OF assms(1)] show ?thesis
+  proof cases
+    case 1
+    then show ?thesis using assms sorry
+  next
+    case (2 \<sigma> X \<alpha>' \<beta>' \<gamma>)
+    then show ?thesis sorry
+  qed
+
+qed
+
+corollary ipda_comp_imp_derivers:
+  assumes "([A \<rightarrow> \<alpha> . \<beta>] # \<rho> @ [init_symbol IPDA], w) \<turnstile>P* ([P.final_state, init_symbol IPDA], [])"
+  obtains v where "Prods G' \<turnstile> [Nt S'] \<Rightarrow>r* hist \<rho> @ Nt A # map Tm v" 
+    "Prods G' \<turnstile> hist \<rho> @ Nt A # map Tm v \<Rightarrow>r hist \<rho> @ \<alpha> @ \<beta> @ map Tm v"
+proof -
+  note ipda_comp_imp_char_comp[OF assms(1)]
+  from char_comp_imp_derivers[OF this] show thesis using that by blast
+qed
+
+
+corollary char_comp_imp_ipda_comp:
+  assumes "([S' \<rightarrow> [] . [Nt S]], \<gamma>) \<turnstile>c* ([A \<rightarrow> \<alpha> . \<beta>], [])"
+  obtains w \<rho> where 
+    "([A \<rightarrow> \<alpha> . \<beta>] # \<rho> @ [init_symbol IPDA], w) \<turnstile>P* ([P.final_state, init_symbol IPDA], [])"
+    "\<gamma> = hist \<rho> @ \<alpha>"
+proof -
+  from char_comp_imp_derivers[OF assms(1)] obtain \<gamma>' w where deriv:
+    "Prods G' \<turnstile> [Nt S'] \<Rightarrow>r* \<gamma>' @ Nt A # map Tm w"
+    "Prods G' \<turnstile> \<gamma>' @ Nt A # map Tm w \<Rightarrow>r \<gamma>' @ \<alpha> @ \<beta> @ map Tm w"
+    "\<gamma> = \<gamma>' @ \<alpha>" by metis
+  moreover from this obtain v where "Prods G' \<turnstile> \<beta> \<Rightarrow>* map Tm v" 
+    using reduced_derived_substring_imp_derives[of G' "\<gamma>' @ \<alpha>" \<beta> "map Tm w", 
+                                        OF _ G'_reduced G'_not_empty] G'_def append.assoc
+    by (metis (no_types, lifting) Cfg.sel(2) derivers_imp_derives rtranclp.rtrancl_into_rtrancl)
+  ultimately show thesis using derivers_imp_ipda_comp that by metis
+qed
+
+
 
 
 end
